update

2016-AFP/AbstractObjects.thy
@@ -41,7 +41,11 @@ section {* Introduction *}
   computational metaphysics, in which different variants of Kurt G{\"o}del's ontological 
   argument were verified resp. falsified \cite{C40,C55}. 
 
-  In this paper we explore an idea to encode, respectively embed,  MRTT in functional type theory. 
+  In this paper we explore an idea to encode, respectively embed, the second-order fragment of  MRTT in 
+  functional type theory.\footnote{In fact, by using polymorphic variants of the various abbreviations
+  we introduce it should be possible to extend the presented approach to full MRTT. However, we
+  have not fully explored this yet. Moreover, relevant problems, as addressed here, already arise in the context 
+  the second-order fragment of MRTT.}. 
   Thereby, we want adapt and extend ideas from the previous, successful embedding of MFTT in functional 
   type theory.
   Our contribution here shall serve as possible starting point for the subsequent
@@ -197,21 +201,17 @@ section {* Preliminaries *}
   @{text "\<^bold>\<A>"} ("it is actually the case that"), refer to a (fixed) designated world. To model such a 
   rigid dependence we introduce a constant symbol (name) @{text "dw"} of world type @{text "i"}. 
   Moreover, for technical reasons, 
-  which will be clarified below, we introduce further (dummy) constant symbols for the various other domains. 
-  We anyway assume that all domains are non-empty. Hence, introducing these constant symbols is obviously not 
-  harmful.\footnote{The single polymorphic dummy @{text "da::'a"}, utilized e.g. in the definition of the universal 
-  quantifier of MRTT below, actually covers already all cases. However, to avoid unnecessary type inferences we
-  actually prefer non-polymorphic dummy elements in all those cases where we can statically 
-  determine the required type.}
+  which will be clarified below, we introduce a polymorphic (dummy) constant symbol @{text "da::'a"} for the various other domains. 
+  We anyway assume that all domains are non-empty. Hence, introducing @{text "da::'a"} is obviously not 
+  harmful.
   *}
 
- consts dw::"i" 
- consts de::"e" dio::"io" deio::"e\<Rightarrow>io" da::"'a"
+ consts dw::"i" da::"'a"
 
 section {* Embedding of Modal Relational Type Theory *}
 
   text {* 
-  The various language constructs of MRTT (see Figure \ref{mmrt}) are now introduced step by step. 
+  The various language constructs of the second-order fragement of MRTT (see Figure \ref{mmrt}) are now introduced step by step. 
   *}
 
   text {* The actuality operator @{text "\<^bold>\<A>"}, when being applied to a formula or propositional formula 
@@ -227,7 +227,7 @@ section {* Embedding of Modal Relational Type Theory *}
  abbreviation Actual::"io opt \<Rightarrow> io opt" ("\<^bold>\<A> _" [64] 65) where "\<^bold>\<A>\<phi> \<equiv> case \<phi> of 
     F(\<psi>) \<Rightarrow> F(\<lambda>w. \<psi> dw) | 
     P(\<psi>) \<Rightarrow> P(\<lambda>w. \<psi> dw) | 
-    _ \<Rightarrow> ERR(dio)"
+    _ \<Rightarrow> ERR(da)"
 
   text {* 
   The Theory of Abstract Objects distinguishes between encoding properties @{text "\<kappa>\<^sub>1\<Pi>\<^sup>1"} and 
@@ -251,9 +251,9 @@ section {* Embedding of Modal Relational Type Theory *}
 
  consts enc::"io\<Rightarrow>io" 
 
- abbreviation Enc::"'a opt\<Rightarrow>('a\<Rightarrow>io) opt\<Rightarrow>io opt" ("\<lbrace>_,_\<rbrace>") where "\<lbrace>x,\<Phi>\<rbrace> \<equiv> case (x,\<Phi>) of 
+ abbreviation Enc::"e opt\<Rightarrow>(e\<Rightarrow>io) opt\<Rightarrow>io opt" ("\<lbrace>_,_\<rbrace>") where "\<lbrace>x,\<Phi>\<rbrace> \<equiv> case (x,\<Phi>) of 
     (T(y),T(Q)) \<Rightarrow> F((enc (Q y))) | 
-    _ \<Rightarrow> ERR(dio)"
+    _ \<Rightarrow> ERR(da)"
 
  text {* We add some exemplary axioms to support reasoning with encodings. Future work will
  be to study and add further principles. *}
@@ -268,9 +268,9 @@ section {* Embedding of Modal Relational Type Theory *}
   *}
 
  (* consts exe::"io\<Rightarrow>io" *)
- abbreviation Exe1::"('a\<Rightarrow>io) opt\<Rightarrow>'a opt\<Rightarrow>io opt" ("\<lparr>_,_\<rparr>") where "\<lparr>\<Phi>,x\<rparr> \<equiv> case (\<Phi>,x) of 
+ abbreviation Exe1::"(e\<Rightarrow>io) opt\<Rightarrow>e opt\<Rightarrow>io opt" ("\<lparr>_,_\<rparr>") where "\<lparr>\<Phi>,x\<rparr> \<equiv> case (\<Phi>,x) of 
     (T(Q),T(y)) \<Rightarrow> P((Q y)) | 
-    _ \<Rightarrow> ERR(dio)"
+    _ \<Rightarrow> ERR(da)"
 
 
   text {* 
@@ -278,14 +278,14 @@ section {* Embedding of Modal Relational Type Theory *}
  In addition to the unary case above, we thus introduce two further cases.
   *}  
 
- abbreviation Exe2::"('a\<Rightarrow>'a\<Rightarrow>io) opt\<Rightarrow>'a opt\<Rightarrow>'a opt\<Rightarrow>io opt" ("\<lparr>_,_,_\<rparr>")
+ abbreviation Exe2::"(e\<Rightarrow>e\<Rightarrow>io) opt\<Rightarrow>e opt\<Rightarrow>e opt\<Rightarrow>io opt" ("\<lparr>_,_,_\<rparr>")
   where "\<lparr>\<Phi>,x1,x2\<rparr> \<equiv> case (\<Phi>,x1,x2) of 
     (T(Q),T(y1),T(y2)) \<Rightarrow> P((Q y1 y2)) | 
-    _ \<Rightarrow> ERR(dio)"
- abbreviation Exe3::"('a\<Rightarrow>'a\<Rightarrow>'a\<Rightarrow>io) opt\<Rightarrow>'a opt\<Rightarrow>'a opt\<Rightarrow>'a opt\<Rightarrow>io opt" ("\<lparr>_,_,_,_\<rparr>") 
+    _ \<Rightarrow> ERR(da)"
+ abbreviation Exe3::"(e\<Rightarrow>e\<Rightarrow>e\<Rightarrow>io) opt\<Rightarrow>e opt\<Rightarrow>e opt\<Rightarrow>e opt\<Rightarrow>io opt" ("\<lparr>_,_,_,_\<rparr>") 
   where "\<lparr>\<Phi>,x1,x2,x3\<rparr> \<equiv> case (\<Phi>,x1,x2,x3) of 
     (T(Q),T(y1),T(y2),T(y3)) \<Rightarrow> P((Q y1 y2 y3)) | 
-    _ \<Rightarrow> ERR(dio)"
+    _ \<Rightarrow> ERR(da)"
 
   text {* 
   Formations with negation and implication are supported for both, formulas and propositional
@@ -298,13 +298,13 @@ section {* Embedding of Modal Relational Type Theory *}
  abbreviation not::"io opt\<Rightarrow>io opt" ("\<^bold>\<not> _" [58] 59) where "\<^bold>\<not> \<phi> \<equiv> case \<phi> of 
     F(\<psi>) \<Rightarrow> F(\<lambda>w.\<not>(\<psi> w)) | 
     P(\<psi>) \<Rightarrow> P(\<lambda>w.\<not>(\<psi> w)) | 
-    _ \<Rightarrow> ERR(dio)"  
+    _ \<Rightarrow> ERR(da)"  
  abbreviation implies::"io opt\<Rightarrow>io opt\<Rightarrow>io opt" (infixl "\<^bold>\<rightarrow>" 51) where "\<phi> \<^bold>\<rightarrow> \<psi> \<equiv> case (\<phi>,\<psi>) of 
     (P(\<alpha>),P(\<beta>)) \<Rightarrow> P(\<lambda>w. \<alpha> w \<longrightarrow> \<beta> w) | 
     (F(\<alpha>),F(\<beta>)) \<Rightarrow> F(\<lambda>w. \<alpha> w \<longrightarrow> \<beta> w) | 
     (P(\<alpha>),F(\<beta>)) \<Rightarrow> F(\<lambda>w. \<alpha> w \<longrightarrow> \<beta> w) | 
     (F(\<alpha>),P(\<beta>)) \<Rightarrow> F(\<lambda>w. \<alpha> w \<longrightarrow> \<beta> w) | 
-    _ \<Rightarrow> ERR(dio)"  
+    _ \<Rightarrow> ERR(da)"  
 
   text {*
   Also universal quantification @{text "\<^bold>\<forall>(\<lambda>x.\<phi>)"} (first-order and higher-order) is supported 
@@ -319,7 +319,7 @@ section {* Embedding of Modal Relational Type Theory *}
  abbreviation forall::"('a\<Rightarrow>io opt)\<Rightarrow>io opt" ("\<^bold>\<forall>") where "\<^bold>\<forall>\<Phi> \<equiv> case (\<Phi> da) of
     F(_) \<Rightarrow> F(\<lambda>w.\<forall>x. case (\<Phi> x) of F(\<psi>) \<Rightarrow> \<psi> w) | 
     P(_) \<Rightarrow> P(\<lambda>w.\<forall>x. case (\<Phi> x) of P(\<psi>) \<Rightarrow> \<psi> w) | 
-    _ \<Rightarrow> ERR(dio)"
+    _ \<Rightarrow> ERR(da)"
  abbreviation forallBinder::"('a\<Rightarrow>io opt)\<Rightarrow>io opt" (binder "\<^bold>\<forall>" [8] 9)  where "\<^bold>\<forall>x. \<phi> x \<equiv> \<^bold>\<forall>\<phi>"
 
 (* lemma binderTest: "(\<^bold>\<forall>x. \<phi> x) = \<^bold>\<forall>(\<lambda>x. \<phi> x)" by simp *)
@@ -337,7 +337,7 @@ section {* Embedding of Modal Relational Type Theory *}
  abbreviation box::"io opt\<Rightarrow>io opt" ("\<^bold>\<box>_" [62] 63) where "\<^bold>\<box>\<phi> \<equiv> case \<phi> of 
     F(\<psi>) \<Rightarrow> F(\<lambda>w.\<forall>v. \<psi> v) | 
     P(\<psi>) \<Rightarrow> P(\<lambda>w.\<forall>v. \<psi> v) | 
-    _ \<Rightarrow> ERR(dio)"  
+    _ \<Rightarrow> ERR(da)"  
 
   text {* 
   n-ary lambda abstraction @{text "\<^bold>\<lambda>\<^sup>0,\<^bold>\<lambda>,\<^bold>\<lambda>\<^sup>2\<^sup>,\<^bold>\<lambda>\<^sup>3,..."}, for $n\geq 0$, is supported in the theory of abstract 
@@ -356,17 +356,17 @@ section {* Embedding of Modal Relational Type Theory *}
 
  abbreviation lam0::"io opt\<Rightarrow>io opt" ("\<^bold>\<lambda>\<^sup>0") where "\<^bold>\<lambda>\<^sup>0\<phi> \<equiv> case \<phi> of 
     P(\<psi>) \<Rightarrow> P(\<psi>) | 
-    _ \<Rightarrow> ERR dio"  
- abbreviation lam::"('a\<Rightarrow>io opt)\<Rightarrow>('a\<Rightarrow>io) opt" ("\<^bold>\<lambda>") where "\<^bold>\<lambda>\<Phi> \<equiv> case (\<Phi> da) of
+    _ \<Rightarrow> ERR da"  
+ abbreviation lam::"(e\<Rightarrow>io opt)\<Rightarrow>(e\<Rightarrow>io) opt" ("\<^bold>\<lambda>") where "\<^bold>\<lambda>\<Phi> \<equiv> case (\<Phi> da) of
     P(_) \<Rightarrow> T(\<lambda>x. case (\<Phi> x) of P(\<phi>) \<Rightarrow> \<phi>) | 
-    _ \<Rightarrow> ERR(\<lambda>x. dio)"
- abbreviation lamBinder::"('a\<Rightarrow>io opt)\<Rightarrow>('a\<Rightarrow>io) opt" (binder "\<^bold>\<lambda>" [8] 9)  where "\<^bold>\<lambda>x. \<phi> x \<equiv> \<^bold>\<lambda> \<phi>"
- abbreviation lam2::"('a\<Rightarrow>'a\<Rightarrow>io opt)\<Rightarrow>('a\<Rightarrow>'a\<Rightarrow>io) opt" ("\<^bold>\<lambda>\<^sup>2") where "\<^bold>\<lambda>\<^sup>2\<Phi> \<equiv> case (\<Phi> da da) of
+    _ \<Rightarrow> ERR(\<lambda>x. da)"
+ abbreviation lamBinder::"(e\<Rightarrow>io opt)\<Rightarrow>(e\<Rightarrow>io) opt" (binder "\<^bold>\<lambda>" [8] 9)  where "\<^bold>\<lambda>x. \<phi> x \<equiv> \<^bold>\<lambda> \<phi>"
+ abbreviation lam2::"(e\<Rightarrow>e\<Rightarrow>io opt)\<Rightarrow>(e\<Rightarrow>e\<Rightarrow>io) opt" ("\<^bold>\<lambda>\<^sup>2") where "\<^bold>\<lambda>\<^sup>2\<Phi> \<equiv> case (\<Phi> da da) of
     P(_) \<Rightarrow> T(\<lambda>x y. case (\<Phi> x y) of P(\<phi>) \<Rightarrow> \<phi>) | 
-    _ \<Rightarrow> ERR(\<lambda>x y. dio)"
- abbreviation lam3::"('a\<Rightarrow>'a\<Rightarrow>'a\<Rightarrow>io opt)\<Rightarrow>('a\<Rightarrow>'a\<Rightarrow>'a\<Rightarrow>io) opt" ("\<^bold>\<lambda>\<^sup>3") where "\<^bold>\<lambda>\<^sup>3\<Phi> \<equiv> case (\<Phi> da da da) of
+    _ \<Rightarrow> ERR(\<lambda>x y. da)"
+ abbreviation lam3::"(e\<Rightarrow>e\<Rightarrow>e\<Rightarrow>io opt)\<Rightarrow>(e\<Rightarrow>e\<Rightarrow>e\<Rightarrow>io) opt" ("\<^bold>\<lambda>\<^sup>3") where "\<^bold>\<lambda>\<^sup>3\<Phi> \<equiv> case (\<Phi> da da da) of
     P(_) \<Rightarrow> T(\<lambda>x y z. case (\<Phi> x y z) of P(\<phi>) \<Rightarrow> \<phi>) | 
-    _ \<Rightarrow> ERR(\<lambda>x y z. dio)"
+    _ \<Rightarrow> ERR(\<lambda>x y z. da)"
 
   text {* 
   The theory of abstract objects supports rigid definite descriptions. Our definition maps
@@ -376,11 +376,11 @@ section {* Embedding of Modal Relational Type Theory *}
   We again introduce binder notation for @{text "\<^bold>\<iota>"}.
   *}
  
- abbreviation that::"('a\<Rightarrow>io opt)\<Rightarrow>'a opt" ("\<^bold>\<iota>")  where "\<^bold>\<iota>\<Phi> \<equiv> case (\<Phi> da) of
+ abbreviation that::"(e\<Rightarrow>io opt)\<Rightarrow>e opt" ("\<^bold>\<iota>")  where "\<^bold>\<iota>\<Phi> \<equiv> case (\<Phi> da) of
     F(_) \<Rightarrow> T(THE x. case (\<Phi> x) of F \<psi> \<Rightarrow> \<psi> dw) | 
     P(_) \<Rightarrow> T(THE x. case (\<Phi> x) of P \<psi> \<Rightarrow> \<psi> dw) | 
     _ \<Rightarrow> ERR(da)"
- abbreviation thatBinder::"('a\<Rightarrow>io opt)\<Rightarrow>'a opt" (binder "\<^bold>\<iota>" [8] 9)  where "\<^bold>\<iota>x. \<phi> x \<equiv> \<^bold>\<iota> \<phi>"
+ abbreviation thatBinder::"(e\<Rightarrow>io opt)\<Rightarrow>e opt" (binder "\<^bold>\<iota>" [8] 9)  where "\<^bold>\<iota>x. \<phi> x \<equiv> \<^bold>\<iota> \<phi>"
 
 
 section {* Further Logical Connectives *}
@@ -392,27 +392,27 @@ section {* Further Logical Connectives *}
  abbreviation conj::"io opt\<Rightarrow>io opt\<Rightarrow>io opt" (infixl "\<^bold>\<and>" 53) where "\<phi> \<^bold>\<and> \<psi> \<equiv> case (\<phi>,\<psi>) of
     (P(\<alpha>),P(\<beta>)) \<Rightarrow> P(\<lambda>w. \<alpha> w \<and> \<beta> w) | (F(\<alpha>),F(\<beta>)) \<Rightarrow> F(\<lambda>w. \<alpha> w \<and> \<beta> w) | 
     (P(\<alpha>),F(\<beta>)) \<Rightarrow> F(\<lambda>w. \<alpha> w \<and> \<beta> w) | (F(\<alpha>),P(\<beta>)) \<Rightarrow> F(\<lambda>w. \<alpha> w \<and> \<beta> w) | 
-    _ \<Rightarrow> ERR(dio)"  
+    _ \<Rightarrow> ERR(da)"  
 
  abbreviation disj::"io opt\<Rightarrow>io opt\<Rightarrow>io opt" (infixl "\<^bold>\<or>" 52) where "\<phi> \<^bold>\<or> \<psi> \<equiv> case (\<phi>,\<psi>) of
     (P(\<alpha>),P(\<beta>)) \<Rightarrow> P(\<lambda>w. \<alpha> w \<or> \<beta> w) | (F(\<alpha>),F(\<beta>)) \<Rightarrow> F(\<lambda>w. \<alpha> w \<or> \<beta> w) | 
     (P(\<alpha>),F(\<beta>)) \<Rightarrow> F(\<lambda>w. \<alpha> w \<or> \<beta> w) | (F(\<alpha>),P(\<beta>)) \<Rightarrow> F(\<lambda>w. \<alpha> w \<or> \<beta> w) | 
-    _ \<Rightarrow> ERR(dio)"  
+    _ \<Rightarrow> ERR(da)"  
 
  abbreviation equiv::"io opt\<Rightarrow>io opt\<Rightarrow>io opt" (infixl "\<^bold>\<equiv>" 51) where "\<phi> \<^bold>\<equiv> \<psi>\<equiv> case (\<phi>,\<psi>) of
     (P(\<alpha>),P(\<beta>)) \<Rightarrow> P(\<lambda>w. \<alpha> w \<longleftrightarrow> \<beta> w) | (F(\<alpha>),F(\<beta>)) \<Rightarrow> F(\<lambda>w. \<alpha> w \<longleftrightarrow> \<beta> w) | 
     (P(\<alpha>),F(\<beta>)) \<Rightarrow> F(\<lambda>w. \<alpha> w \<longleftrightarrow> \<beta> w) | (F(\<alpha>),P(\<beta>)) \<Rightarrow> F(\<lambda>w. \<alpha> w \<longleftrightarrow> \<beta> w) | 
-    _ \<Rightarrow> ERR(dio)"  
+    _ \<Rightarrow> ERR(da)"  
 
  abbreviation diamond::"io opt\<Rightarrow>io opt" ("\<^bold>\<diamond> _" [62] 63) where "\<^bold>\<diamond>\<phi> \<equiv> case \<phi> of 
     F(\<psi>) \<Rightarrow> F(\<lambda>w.\<exists>v. \<psi> v) | 
     P(\<psi>) \<Rightarrow> P(\<lambda>w.\<exists>v. \<psi> v) | 
-    _ \<Rightarrow> ERR(dio)"
+    _ \<Rightarrow> ERR(da)"
 
  abbreviation exists::"('a\<Rightarrow>io opt)\<Rightarrow>io opt" ("\<^bold>\<exists>") where "\<^bold>\<exists>\<Phi> \<equiv> case (\<Phi> da) of
     P(_) \<Rightarrow> P(\<lambda>w.\<exists>x. case (\<Phi> x) of P \<psi> \<Rightarrow> \<psi> w) | 
     F(_) \<Rightarrow> F(\<lambda>w. \<exists>x. case (\<Phi> x) of F \<psi> \<Rightarrow> \<psi> w) | 
-    _ \<Rightarrow> ERR dio" 
+    _ \<Rightarrow> ERR da" 
  abbreviation existsBinder::"('a\<Rightarrow>io opt)\<Rightarrow>io opt" (binder "\<^bold>\<exists>" [8] 9)  where "\<^bold>\<exists>x. \<phi> x \<equiv> \<^bold>\<exists>\<phi>"
 
 section {* E!, O!, A! and =E *}
@@ -422,41 +422,41 @@ section {* E!, O!, A! and =E *}
   start out with the distinguished 1-place relation constant @{text "E!"} (read ‘being concrete’ or ‘concreteness’). 
   *}
 
- consts Exists::"('a\<Rightarrow>io)" ("E!")
+ consts Exists::"(e\<Rightarrow>io)" ("E!")
  
   text {* 
   Next, being ordinary is defined as being possibly concrete. 
   *}
 
- abbreviation ordinaryObject::"('a\<Rightarrow>io) opt" ("O!") where "O! \<equiv> \<^bold>\<lambda>x. \<^bold>\<diamond>\<lparr>E!\<^sup>T,x\<^sup>T\<rparr>"
+ abbreviation ordinaryObject::"(e\<Rightarrow>io) opt" ("O!") where "O! \<equiv> \<^bold>\<lambda>x. \<^bold>\<diamond>\<lparr>E!\<^sup>T,x\<^sup>T\<rparr>"
 
   text {* 
   Being abstract is then defined as not possibly being concrete. 
   *}
 
- abbreviation abstractObject::"('a\<Rightarrow>io) opt" ("A!") where "A! \<equiv> \<^bold>\<lambda>x. \<^bold>\<not>(\<^bold>\<diamond>\<lparr>E!\<^sup>T,x\<^sup>T\<rparr>)"
+ abbreviation abstractObject::"(e\<Rightarrow>io) opt" ("A!") where "A! \<equiv> \<^bold>\<lambda>x. \<^bold>\<not>(\<^bold>\<diamond>\<lparr>E!\<^sup>T,x\<^sup>T\<rparr>)"
 
   text {* 
   Finally, we introduce the identity relations @{text "\<^bold>=\<^sub>E"} and @{text "\<^bold>="} on individuals. 
   *}
 
- abbreviation identityE::"'a opt\<Rightarrow>'a opt\<Rightarrow>io opt" (infixl "\<^bold>=\<^sub>E" 63) where "x \<^bold>=\<^sub>E y \<equiv> 
+ abbreviation identityE::"e opt\<Rightarrow>e opt\<Rightarrow>io opt" (infixl "\<^bold>=\<^sub>E" 63) where "x \<^bold>=\<^sub>E y \<equiv> 
     \<lparr>O!,x\<rparr> \<^bold>\<and> \<lparr>O!,y\<rparr> \<^bold>\<and> \<^bold>\<box>(\<^bold>\<forall>F. \<lparr>F\<^sup>T,x\<rparr> \<^bold>\<equiv> \<lparr>F\<^sup>T,y\<rparr>)"
 
- abbreviation identityI::"'a opt\<Rightarrow>'a opt\<Rightarrow>io opt" (infixl "\<^bold>=" 63) where "x \<^bold>= y \<equiv> 
+ abbreviation identityI::"e opt\<Rightarrow>e opt\<Rightarrow>io opt" (infixl "\<^bold>=" 63) where "x \<^bold>= y \<equiv> 
     x \<^bold>=\<^sub>E y \<^bold>\<or> (\<lparr>A!,x\<rparr> \<^bold>\<and> \<lparr>A!,y\<rparr> \<^bold>\<and> \<^bold>\<box>(\<^bold>\<forall>F. \<lbrace>x,F\<^sup>T\<rbrace> \<^bold>\<equiv> \<lbrace>y,F\<^sup>T\<rbrace>))"
 
 
  text {* Moreover, we introduce the following identity relations on n-ary relations (for $n=0,1,2,3$). *}
 
- abbreviation identityRel1::" (('a\<Rightarrow>io) opt)\<Rightarrow>(('a\<Rightarrow>io) opt)\<Rightarrow>io opt" (infixl "\<^bold>=\<^sup>1" 63) 
+ abbreviation identityRel1::" ((e\<Rightarrow>io) opt)\<Rightarrow>((e\<Rightarrow>io) opt)\<Rightarrow>io opt" (infixl "\<^bold>=\<^sup>1" 63) 
    where "F1 \<^bold>=\<^sup>1 G1 \<equiv> \<^bold>\<box>(\<^bold>\<forall>x. \<lbrace>x\<^sup>T,F1\<rbrace> \<^bold>\<equiv> \<lbrace>x\<^sup>T,G1\<rbrace>)"
 
- abbreviation identityRel2::" (('a\<Rightarrow>'a\<Rightarrow>io) opt)\<Rightarrow>(('a\<Rightarrow>'a\<Rightarrow>io) opt)\<Rightarrow>io opt" (infixl "\<^bold>=\<^sup>2" 63) 
+ abbreviation identityRel2::" ((e\<Rightarrow>e\<Rightarrow>io) opt)\<Rightarrow>((e\<Rightarrow>e\<Rightarrow>io) opt)\<Rightarrow>io opt" (infixl "\<^bold>=\<^sup>2" 63) 
    where "F2 \<^bold>=\<^sup>2 G2 \<equiv> \<^bold>\<forall>x1.(  (\<^bold>\<lambda>y.\<lparr>F2,y\<^sup>T,x1\<^sup>T\<rparr>) \<^bold>=\<^sup>1 (\<^bold>\<lambda>y.\<lparr>G2,y\<^sup>T,x1\<^sup>T\<rparr>)
                           \<^bold>\<and> (\<^bold>\<lambda>y.\<lparr>F2,x1\<^sup>T,y\<^sup>T\<rparr>) \<^bold>=\<^sup>1 (\<^bold>\<lambda>y.\<lparr>G2,x1\<^sup>T,y\<^sup>T\<rparr>))"
 
- abbreviation identityRel3::" (('a\<Rightarrow>'a\<Rightarrow>'a\<Rightarrow>io) opt)\<Rightarrow>(('a\<Rightarrow>'a\<Rightarrow>'a\<Rightarrow>io) opt)\<Rightarrow>io opt" (infixl "\<^bold>=\<^sup>3" 63) 
+ abbreviation identityRel3::" ((e\<Rightarrow>e\<Rightarrow>e\<Rightarrow>io) opt)\<Rightarrow>((e\<Rightarrow>e\<Rightarrow>e\<Rightarrow>io) opt)\<Rightarrow>io opt" (infixl "\<^bold>=\<^sup>3" 63) 
    where "F3 \<^bold>=\<^sup>3 G3 \<equiv> \<^bold>\<forall>x1 x2.(  (\<^bold>\<lambda>y.\<lparr>F3,y\<^sup>T,x1\<^sup>T,x2\<^sup>T\<rparr>) \<^bold>=\<^sup>1 (\<^bold>\<lambda>y.\<lparr>G3,y\<^sup>T,x1\<^sup>T,x2\<^sup>T\<rparr>)
                              \<^bold>\<and> (\<^bold>\<lambda>y.\<lparr>F3,x1\<^sup>T,y\<^sup>T,x2\<^sup>T\<rparr>) \<^bold>=\<^sup>1 (\<^bold>\<lambda>y.\<lparr>G3,x1\<^sup>T,y\<^sup>T,x2\<^sup>T\<rparr>)
                              \<^bold>\<and> (\<^bold>\<lambda>y.\<lparr>F3,x1\<^sup>T,x2\<^sup>T,y\<^sup>T\<rparr>) \<^bold>=\<^sup>1 (\<^bold>\<lambda>y.\<lparr>G3,x1\<^sup>T,x2\<^sup>T,y\<^sup>T\<rparr>))"
@@ -488,8 +488,8 @@ section {* Three-Valued Meta-Logic*}
   we only use validity.
   *}
 
- (*<*) no_syntax "_list" :: "args \<Rightarrow> 'a list" ("[(_)]") (*>*) 
- (*<*) no_syntax "__listcompr" :: "args \<Rightarrow> 'a list" ("[(_)]") (*>*) 
+ (*<*) no_syntax "_list" :: "args \<Rightarrow> e list" ("[(_)]") (*>*) 
+ (*<*) no_syntax "__listcompr" :: "args \<Rightarrow> e list" ("[(_)]") (*>*) 
  abbreviation valid :: "io opt\<Rightarrow>mf" ("[_]" [1]) where "[\<phi>] \<equiv> case \<phi> of 
     P(\<psi>) \<Rightarrow> if \<forall>w.(\<psi> w) \<longleftrightarrow> True then \<top> else \<bottom> | 
     F(\<psi>) \<Rightarrow> if \<forall>w.(\<psi> w) \<longleftrightarrow> True then \<top> else \<bottom> | 
@@ -527,18 +527,18 @@ section {* Some Tests and First Applications*}
     actual internal term  
    @{text "(case case case \<lbrace>da\<^sup>T,da\<^sup>T\<rbrace> \<^bold>\<rightarrow> \<lparr>da\<^sup>T,da\<^sup>T\<rparr> of
                P x \<Rightarrow> (\<lambda>w. \<forall>x. case \<lbrace>x\<^sup>T,da\<^sup>T\<rbrace> \<^bold>\<rightarrow> \<lparr>da\<^sup>T,x\<^sup>T\<rparr> of P \<psi> \<Rightarrow> \<psi> w)\<^sup>P
-               | F x \<Rightarrow> (\<lambda>w. \<forall>x. case \<lbrace>x\<^sup>T,da\<^sup>T\<rbrace> \<^bold>\<rightarrow> \<lparr>da\<^sup>T,x\<^sup>T\<rparr> of F \<psi> \<Rightarrow> \<psi> w)\<^sup>F | _ \<Rightarrow> dio\<^sup>E of
+               | F x \<Rightarrow> (\<lambda>w. \<forall>x. case \<lbrace>x\<^sup>T,da\<^sup>T\<rbrace> \<^bold>\<rightarrow> \<lparr>da\<^sup>T,x\<^sup>T\<rparr> of F \<psi> \<Rightarrow> \<psi> w)\<^sup>F | _ \<Rightarrow> da\<^sup>E of
           P x \<Rightarrow> (\<lambda>w. \<forall>x. case case \<lbrace>da\<^sup>T,x\<^sup>T\<rbrace> \<^bold>\<rightarrow> \<lparr>x\<^sup>T,da\<^sup>T\<rparr> of
                                P xa \<Rightarrow> (\<lambda>w. \<forall>xa. case \<lbrace>xa\<^sup>T,x\<^sup>T\<rbrace> \<^bold>\<rightarrow> \<lparr>x\<^sup>T,xa\<^sup>T\<rparr> of P \<psi> \<Rightarrow> \<psi> w)\<^sup>P
                                | F xa \<Rightarrow> (\<lambda>w. \<forall>xa. case \<lbrace>xa\<^sup>T,x\<^sup>T\<rbrace> \<^bold>\<rightarrow> \<lparr>x\<^sup>T,xa\<^sup>T\<rparr> of F \<psi> \<Rightarrow> \<psi> w)\<^sup>F
-                               | _ \<Rightarrow> dio\<^sup>E of
+                               | _ \<Rightarrow> da\<^sup>E of
                           P \<psi> \<Rightarrow> \<psi> w)\<^sup>P
           | F x \<Rightarrow> (\<lambda>w. \<forall>x. case case \<lbrace>da\<^sup>T,x\<^sup>T\<rbrace> \<^bold>\<rightarrow> \<lparr>x\<^sup>T,da\<^sup>T\<rparr> of
                                  P xa \<Rightarrow> (\<lambda>w. \<forall>xa. case \<lbrace>xa\<^sup>T,x\<^sup>T\<rbrace> \<^bold>\<rightarrow> \<lparr>x\<^sup>T,xa\<^sup>T\<rparr> of P \<psi> \<Rightarrow> \<psi> w)\<^sup>P
                                  | F xa \<Rightarrow> (\<lambda>w. \<forall>xa. case \<lbrace>xa\<^sup>T,x\<^sup>T\<rbrace> \<^bold>\<rightarrow> \<lparr>x\<^sup>T,xa\<^sup>T\<rparr> of F \<psi> \<Rightarrow> \<psi> w)\<^sup>F
-                                 | _ \<Rightarrow> dio\<^sup>E of
+                                 | _ \<Rightarrow> da\<^sup>E of
                             F \<psi> \<Rightarrow> \<psi> w)\<^sup>F
-          | _ \<Rightarrow> dio\<^sup>E of
+          | _ \<Rightarrow> da\<^sup>E of
      P \<psi> \<Rightarrow> if \<forall>w. \<psi> w = True then \<top> else \<bottom> | F \<psi> \<Rightarrow> if \<forall>w. \<psi> w = True then \<top> else \<bottom> | _ \<Rightarrow> *) =
     \<top>"}.
   In Isabelle the inflated term is displayed in the output window when placing the mouse on the abbreviated representation.
@@ -630,11 +630,11 @@ section {* Some Tests and First Applications*}
  The expression @{text "(\<^bold>\<lambda>x. \<^bold>\<exists>F. \<lbrace>x\<^sup>T,F\<^sup>T\<rbrace> \<^bold>\<and> \<^bold>\<not>\<lparr>F\<^sup>T,x\<^sup>T\<rparr>)"} is an ineligible 
  construct, cf.~\cite[chap.4]{zalta11:_relat_versus_funct_found_logic}. 
  When placing the
- mouse on 'simp' we see that this is evaluated to @{text "(\<lambda>x. dio)\<^sup>E"} as intended, i.e. an ERR-term
+ mouse on 'simp' we see that this is evaluated to @{text "(\<lambda>x. da)\<^sup>E"} as intended, i.e. an ERR-term
  is returned.  
  *}
 
- lemma "(\<^bold>\<lambda>x. \<^bold>\<exists>F. \<lbrace>x\<^sup>T,F\<^sup>T\<rbrace> \<^bold>\<and> \<^bold>\<not>\<lparr>F\<^sup>T,x\<^sup>T\<rparr>) = X" apply simp oops  -- {* X is @{text "(\<lambda>x. dio)\<^sup>E"} *}
+ lemma "(\<^bold>\<lambda>x. \<^bold>\<exists>F. \<lbrace>x\<^sup>T,F\<^sup>T\<rbrace> \<^bold>\<and> \<^bold>\<not>\<lparr>F\<^sup>T,x\<^sup>T\<rparr>) = X" apply simp oops  -- {* X is @{text "(\<lambda>x. da)\<^sup>E"} *}
 
  text {*   
   Similarly, the following comprehension principle for abstract objects is an ineligible formula,  
@@ -676,6 +676,7 @@ cf. ~\cite[chap.4]{zalta11:_relat_versus_funct_found_logic} *}
 
  subsection {* Properties of Equality *}
 
+(*
  lemma "[(\<^bold>\<forall>x y. (x\<^sup>T \<^bold>= x\<^sup>T))] = \<top>" apply simp by blast
  lemma "[(\<^bold>\<forall>x y. x\<^sup>T \<^bold>= y\<^sup>T \<^bold>\<rightarrow> y\<^sup>T \<^bold>= x\<^sup>T)] = \<top>" apply simp by meson
  lemma "[(\<^bold>\<forall>x y z. (x\<^sup>T \<^bold>= y\<^sup>T \<^bold>\<and> y\<^sup>T \<^bold>= z\<^sup>T) \<^bold>\<rightarrow> x\<^sup>T \<^bold>= z\<^sup>T)] = \<top>" apply simp  by meson 
@@ -706,7 +707,7 @@ cf. ~\cite[chap.4]{zalta11:_relat_versus_funct_found_logic} *}
  lemma "[(\<^bold>\<forall>x y. x\<^sup>T \<^bold>=\<^sup>3 y\<^sup>T \<^bold>\<rightarrow> y\<^sup>T \<^bold>=\<^sup>3 x\<^sup>T)] = \<top>" apply simp done
  lemma "[(\<^bold>\<forall>x y z. (x\<^sup>T \<^bold>=\<^sup>3 y\<^sup>T \<^bold>\<and> y\<^sup>T \<^bold>=\<^sup>3 z\<^sup>T) \<^bold>\<rightarrow> x\<^sup>T \<^bold>=\<^sup>3 z\<^sup>T)] = \<top>" apply simp done
  lemma "[(\<^bold>\<forall>x y. x\<^sup>T \<^bold>=\<^sup>3 y\<^sup>T \<^bold>\<rightarrow> \<^bold>\<box>(x\<^sup>T \<^bold>=\<^sup>3 y\<^sup>T))] = \<top>" apply simp done 
-
+*)
 
  subsection {* Technological Problem --- Pushing Isabelle to its Limits *} 
 
@@ -751,11 +752,48 @@ cf. ~\cite[chap.4]{zalta11:_relat_versus_funct_found_logic} *}
  text {* Some tests related to beta-conversion. *}
 
  lemma "[(\<^bold>\<forall>z. \<lparr>(\<^bold>\<lambda>y. (\<lparr>Q\<^sup>T,y\<^sup>T\<rparr> \<^bold>\<and> (p\<^sup>P \<^bold>\<or> \<^bold>\<not>p\<^sup>P))),z\<^sup>T\<rparr> \<^bold>\<equiv> \<lparr>(\<^bold>\<lambda>y. (\<lparr>Q\<^sup>T,y\<^sup>T\<rparr> \<^bold>\<and> (q\<^sup>P \<^bold>\<or> \<^bold>\<not>q\<^sup>P))),z\<^sup>T\<rparr>)] = \<top>" apply simp done
- lemma "[(\<^bold>\<lambda>y. (\<lparr>Q\<^sup>T,y\<^sup>T\<rparr> \<^bold>\<and> (q\<^sup>P \<^bold>\<or> \<^bold>\<not>q\<^sup>P))) \<^bold>=\<^sup>1 (\<^bold>\<lambda>y. (\<lparr>Q\<^sup>T,y\<^sup>T\<rparr> \<^bold>\<and> (p\<^sup>P \<^bold>\<or> \<^bold>\<not>p\<^sup>P)))] = \<top>" apply simp done
- lemma "[\<lbrace>x\<^sup>T,(\<^bold>\<lambda>y. (\<lparr>Q\<^sup>T,y\<^sup>T\<rparr> \<^bold>\<and> (q\<^sup>P \<^bold>\<or> \<^bold>\<not>q\<^sup>P)))\<rbrace> \<^bold>\<rightarrow> \<lbrace>x\<^sup>T,(\<^bold>\<lambda>y. (\<lparr>Q\<^sup>T,y\<^sup>T\<rparr> \<^bold>\<and> (p\<^sup>P \<^bold>\<or> \<^bold>\<not>p\<^sup>P)))\<rbrace>] = \<top>" apply simp done
- lemma "[\<lbrace>x\<^sup>T,(\<^bold>\<lambda>y. (\<lparr>Q\<^sup>T,y\<^sup>T\<rparr> \<^bold>\<and> (q\<^sup>P \<^bold>\<or> \<^bold>\<not>q\<^sup>P)))\<rbrace> \<^bold>\<rightarrow> \<lbrace>x\<^sup>T,(\<^bold>\<lambda>z. (\<lparr>Q\<^sup>T,z\<^sup>T\<rparr> \<^bold>\<and> (p\<^sup>P \<^bold>\<or> \<^bold>\<not>p\<^sup>P)))\<rbrace>] = \<top>" apply simp done
 
+ lemma "[(\<^bold>\<lambda>y. (\<lparr>Q\<^sup>T,y\<^sup>T\<rparr> \<^bold>\<and> (q\<^sup>P \<^bold>\<or> \<^bold>\<not>q\<^sup>P))) \<^bold>=\<^sup>1 (\<^bold>\<lambda>y. (\<lparr>Q\<^sup>T,y\<^sup>T\<rparr> \<^bold>\<and> (p\<^sup>P \<^bold>\<or> \<^bold>\<not>p\<^sup>P)))] = \<top>" apply simp done
+ lemma "[(\<^bold>\<lambda>y. (\<lparr>Q\<^sup>T,y\<^sup>T\<rparr> \<^bold>\<and> (q\<^sup>P \<^bold>\<or> \<^bold>\<not>q\<^sup>P))) \<^bold>=\<^sup>1 (\<^bold>\<lambda>z. (\<lparr>Q\<^sup>T,z\<^sup>T\<rparr> \<^bold>\<and> (p\<^sup>P \<^bold>\<or> \<^bold>\<not>p\<^sup>P)))] = \<top>" apply simp done
+
+
+ subsection {* Serious Problem: Boolean Extensionality. \label{booleanExtensionaliy} *}
+
+ text {* The following should not hold in object theory, but it 
+ it is provable in our embedding. Boolean extensionality is exploited by the simplifier.  *}
+
+ lemma "[\<lbrace>x\<^sup>T,(\<^bold>\<lambda>y. (\<lparr>Q\<^sup>T,y\<^sup>T\<rparr> \<^bold>\<and> (q\<^sup>P \<^bold>\<or> \<^bold>\<not>q\<^sup>P)))\<rbrace> \<^bold>\<rightarrow> \<lbrace>x\<^sup>T,(\<^bold>\<lambda>y. (\<lparr>Q\<^sup>T,y\<^sup>T\<rparr> \<^bold>\<and> (p\<^sup>P \<^bold>\<or> \<^bold>\<not>p\<^sup>P)))\<rbrace>] = \<top>" apply simp done
+
+ text {* The reason obviously is that the simplifier of Isabelle detects that 
+ @{text "(q\<^sup>P \<^bold>\<or> \<^bold>\<not>q\<^sup>P)"} and @{text "(p\<^sup>P \<^bold>\<or> \<^bold>\<not>p\<^sup>P)"} both denote truth. 
+ Thus, it simplifies/rewrites both sides of the implication into identical terms. 
+ The statement remains provable even if we slightly modify it (alpha-renaming).
+*}
+
+ lemma "[\<lbrace>x\<^sup>T,(\<^bold>\<lambda>y. (\<lparr>Q\<^sup>T,y\<^sup>T\<rparr> \<^bold>\<and> (q\<^sup>P \<^bold>\<or> \<^bold>\<not>q\<^sup>P)))\<rbrace> \<^bold>\<rightarrow> \<lbrace>x\<^sup>T,(\<^bold>\<lambda>z. (\<lparr>Q\<^sup>T,z\<^sup>T\<rparr> \<^bold>\<and> (p\<^sup>P \<^bold>\<or> \<^bold>\<not>p\<^sup>P)))\<rbrace>] = \<top>" apply simp done
  
+ text {* This is because we also can prove: *}
+
+ lemma "[\<lbrace>x\<^sup>T,(\<^bold>\<lambda>y. \<lparr>Q\<^sup>T,y\<^sup>T\<rparr>)\<rbrace> \<^bold>\<rightarrow> \<lbrace>x\<^sup>T,(\<^bold>\<lambda>z. \<lparr>Q\<^sup>T,z\<^sup>T\<rparr>)\<rbrace>] = \<top>" apply simp done
+
+ text {* In general, we do not want that the following inference holds. This is in fact the 
+  case and Nitpick finds a countermodel. *}
+ (* Ed: From xF and  \<box>\<forall>x(Fx \<rightarrow> Gx)  you can't infer xG *)
+
+ lemma "[(\<lbrace>x\<^sup>T,Q\<^sup>T\<rbrace> \<^bold>\<and> (\<^bold>\<box>(\<^bold>\<forall>x. (\<lparr>Q\<^sup>T,x\<^sup>T\<rparr> \<^bold>\<rightarrow> \<lparr>G\<^sup>T,x\<^sup>T\<rparr>)))) \<^bold>\<rightarrow> \<lbrace>x\<^sup>T,G\<^sup>T\<rbrace>] = \<top>" apply simp 
+   nitpick [user_axioms, expect = genuine, format = 2] oops
+
+ text {* The following should again be provable. This is in line with our approach and confirmed
+  by the provers. *}
+ (* Ed: But from xF and F=G you can infer xG. *)  
+
+ lemma "[(\<lbrace>x\<^sup>T,Q\<^sup>T\<rbrace> \<^bold>\<and> Q\<^sup>T \<^bold>=\<^sup>1 G\<^sup>T) \<^bold>\<rightarrow> \<lbrace>x\<^sup>T,G\<^sup>T\<rbrace>] = \<top>" apply simp by auto
+ 
+ text {* Summary: At this point I have no idea whether the above issue with Boolean extensionality
+  can be saved. How can we block Boolean extensionality from being applied in the above 
+  situation in our framework? *}
+
+
  subsection{* Theory of Encoding *}
 
  text {* We present a small case study in the theory of encoding. For this we first
@@ -766,13 +804,13 @@ cf. ~\cite[chap.4]{zalta11:_relat_versus_funct_found_logic} *}
   OrdinaryObjectsDoNotEncode: "[\<lparr>O!,x\<^sup>T\<rparr> \<^bold>\<rightarrow> \<^bold>\<box>(\<^bold>\<not>(\<^bold>\<exists>F. \<lbrace>x\<^sup>T,F\<^sup>T\<rbrace>))] = \<top>" and
   ObjectComprehension: "[(\<^bold>\<exists>x. \<lparr>A!,x\<^sup>T\<rparr> \<^bold>\<and> (\<^bold>\<forall>F. \<lbrace>x\<^sup>T,F\<^sup>T\<rbrace> \<^bold>\<equiv> \<phi>))] = \<top>"
 
- abbreviation Situation::"'a opt\<Rightarrow>io opt"  where 
+ abbreviation Situation::"e opt\<Rightarrow>io opt"  where 
    "Situation x \<equiv> (\<lparr>A!,x\<rparr> \<^bold>\<and> (\<^bold>\<forall>F. (\<lbrace>x,F\<^sup>T\<rbrace> \<^bold>\<rightarrow> (\<^bold>\<exists>p. F\<^sup>T \<^bold>=\<^sup>1 (\<^bold>\<lambda>y. p\<^sup>P)))))"
- abbreviation PIsTrueInX::"'a opt \<Rightarrow> (i \<Rightarrow> bool) opt \<Rightarrow> (i \<Rightarrow> bool) opt" (infixl "\<Turnstile>" 63) where 
+ abbreviation PIsTrueInX::"e opt \<Rightarrow> (i \<Rightarrow> bool) opt \<Rightarrow> (i \<Rightarrow> bool) opt" (infixl "\<Turnstile>" 63) where 
    "x \<Turnstile> p \<equiv> \<lbrace>x,(\<^bold>\<lambda>y. p)\<rbrace>"  
- abbreviation PossibleWorld::"'a opt\<Rightarrow>io opt" where 
+ abbreviation PossibleWorld::"e opt\<Rightarrow>io opt" where 
    "PossibleWorld x \<equiv> Situation(x) \<^bold>\<and> \<^bold>\<diamond>(\<^bold>\<forall>p. (x \<Turnstile> p\<^sup>P) \<^bold>\<equiv> p\<^sup>P)" 
- abbreviation Maximal::"'a opt\<Rightarrow>io opt" where 
+ abbreviation Maximal::"e opt\<Rightarrow>io opt" where 
    "Maximal s \<equiv> (\<^bold>\<forall>p. (s \<Turnstile> p\<^sup>P) \<^bold>\<or> (s \<Turnstile> (\<^bold>\<not> p\<^sup>P)))" 
 
  text {* We are now in the position to formalize and prove the fundamental theorem of possible worlds,
@@ -793,7 +831,7 @@ cf. ~\cite[chap.4]{zalta11:_relat_versus_funct_found_logic} *}
 
 section {* Conclusion *}
 text {*
-  We have experimented with an new idea towards a shallow embedding of MRTT in 
+  We have experimented with an idea towards a shallow embedding of MRTT in 
   functional type theory 
   and we have pushed the technical 
   elaboration of that idea to some interesting intermediate state.   
@@ -811,6 +849,9 @@ internal formula representing the transitivity of equality between ternary relat
  experiments is reaching an interesting level; cf. the experiments in related work where 
  a significant amount of handselected instantiations of schemata was needed (e.g. for comprehension and lambda
  conversion) \cite{FitelsonZ07,Zalta15}.
+
+ More problematic is the challenge to restrict Boolean extensionality; we briefly discussed the issue by an example 
+ in Subsection \ref{booleanExtensionality}. 
 
  Independent of the outcome of the further research based upon the presented embedding it should 
  become clear that building a system similar to Isabelle but with taking MRTT as its foundational 
